Syntax.thy
@@ -5,11 +5,16 @@ begin
 atom_decl "var"
 atom_decl "tyvar"
 
+nominal_datatype "\<kappa>" =
+  Star ("\<star>")
+  | KArrow "\<kappa>" "\<kappa>"
+
 nominal_datatype "\<tau>" =
   TyUnit
   | TyVar "tyvar"
   | TyArrow "\<tau>" "\<tau>"  ("_ \<rightarrow> _" 50)
-  | TyForall a::"tyvar" t::"\<tau>" binds a in t ("\<forall> _ . _" 50)
+  | TyConApp "\<tau>" "\<tau>"
+  | TyForall a::"tyvar" "\<kappa>" t::"\<tau>" binds a in t ("\<forall> _ : _ . _" 50)
 
 nominal_datatype "term" =
    Var "var"
@@ -17,16 +22,21 @@ nominal_datatype "term" =
  | TyApp "term" "\<tau>"
  | Unit
  | Lam x::"var" "\<tau>" e::"term" binds x in e  ("\<lambda> _ : _ . _" 50)
- | TyLam a::"tyvar" e::"term" binds a in e ("\<Lambda> _ . _" 50)
+ | TyLam a::"tyvar" "\<kappa>" e::"term" binds a in e ("\<Lambda> _ : _ . _" 50)
  | Let x::"var" "\<tau>" "term" e2::"term" binds x in e2
 
 nominal_datatype "binder" =
   "BVar" "var" "\<tau>"
-  | "BTyVar" "tyvar"
+  | "BTyVar" "tyvar" "\<kappa>"
 
 type_synonym "\<Gamma>" = "binder list"
 
+lemma no_vars_in_kinds[simp]: "atom (x :: var) \<sharp> (k :: \<kappa>)"
+  by (induction k rule: \<kappa>.induct) auto
 lemma no_vars_in_ty[simp]: "atom (x :: var) \<sharp> (ty :: \<tau>)"
   by (induction ty rule: \<tau>.induct) auto
+
+lemma no_tyvars_in_kinds[simp]: "atom (a :: tyvar) \<sharp> (k :: \<kappa>)"
+  by (induction k rule: \<kappa>.induct) auto
 
 end
