Typing.thy
@@ -2,14 +2,16 @@ theory Typing
   imports Syntax Defs
 begin
 
-inductive Ty :: "\<Gamma> \<Rightarrow> \<tau> \<Rightarrow> bool" ("_ \<turnstile>\<^sub>t\<^sub>y _") where
-  Ty_Unit: "\<Gamma> \<turnstile>\<^sub>t\<^sub>y TyUnit"
+inductive Ty :: "\<Gamma> \<Rightarrow> \<tau> \<Rightarrow> \<kappa> \<Rightarrow> bool" ("_ \<turnstile>\<^sub>t\<^sub>y _ : _") where
+  Ty_Unit: "\<Gamma> \<turnstile>\<^sub>t\<^sub>y TyUnit : \<star>"
 
-| Ty_Var: "\<lbrakk> BTyVar a \<in> \<Gamma> \<rbrakk> \<Longrightarrow> \<Gamma> \<turnstile>\<^sub>t\<^sub>y TyVar a"
+| Ty_Var: "BTyVar a k \<in> \<Gamma> \<Longrightarrow> \<Gamma> \<turnstile>\<^sub>t\<^sub>y TyVar a : k"
 
-| Ty_Arrow: "\<lbrakk> \<Gamma> \<turnstile>\<^sub>t\<^sub>y \<tau>1 ; \<Gamma> \<turnstile>\<^sub>t\<^sub>y \<tau>2 \<rbrakk> \<Longrightarrow> \<Gamma> \<turnstile>\<^sub>t\<^sub>y (\<tau>1 \<rightarrow> \<tau>2)"
+| Ty_Arrow: "\<lbrakk> \<Gamma> \<turnstile>\<^sub>t\<^sub>y \<tau>1 : \<star> ; \<Gamma> \<turnstile>\<^sub>t\<^sub>y \<tau>2 : \<star> \<rbrakk> \<Longrightarrow> \<Gamma> \<turnstile>\<^sub>t\<^sub>y (\<tau>1 \<rightarrow> \<tau>2) : \<star>"
 
-| Ty_Forall: "\<lbrakk> BTyVar a # \<Gamma> \<turnstile>\<^sub>t\<^sub>y \<sigma> ; atom a \<sharp> \<Gamma> \<rbrakk> \<Longrightarrow> \<Gamma> \<turnstile>\<^sub>t\<^sub>y (\<forall>a. \<sigma>)"
+| Ty_App: "\<lbrakk> \<Gamma> \<turnstile>\<^sub>t\<^sub>y \<tau>1 : KArrow \<kappa>1 \<kappa>2 ; \<Gamma> \<turnstile>\<^sub>t\<^sub>y \<tau>2 : \<kappa>1 \<rbrakk> \<Longrightarrow> \<Gamma> \<turnstile>\<^sub>t\<^sub>y TyConApp \<tau>1 \<tau>2 : \<kappa>2"
+
+| Ty_Forall: "\<lbrakk> BTyVar a k # \<Gamma> \<turnstile>\<^sub>t\<^sub>y \<sigma> : \<star> ; atom a \<sharp> \<Gamma> \<rbrakk> \<Longrightarrow> \<Gamma> \<turnstile>\<^sub>t\<^sub>y (\<forall>a : k. \<sigma>) : \<star>"
 equivariance Ty
 nominal_inductive Ty avoids
   Ty_Forall: a
@@ -20,15 +22,15 @@ inductive T :: "\<Gamma> \<Rightarrow> term \<Rightarrow> \<tau> \<Rightarrow> b
 
 | T_VarI: "\<lbrakk> BVar x \<tau> \<in> \<Gamma> \<rbrakk> \<Longrightarrow> \<Gamma> \<turnstile> (Var x) : \<tau>"
 
-| T_AbsI: "\<lbrakk> atom x \<sharp> \<Gamma> ; \<Gamma> \<turnstile>\<^sub>t\<^sub>y \<tau>1 ; BVar x \<tau>1 # \<Gamma> \<turnstile> e : \<tau>2 \<rbrakk> \<Longrightarrow> \<Gamma> \<turnstile> (\<lambda> x : \<tau>1 . e) : (\<tau>1 \<rightarrow> \<tau>2)"
+| T_AbsI: "\<lbrakk> atom x \<sharp> \<Gamma> ; \<Gamma> \<turnstile>\<^sub>t\<^sub>y \<tau>1 : \<star> ; BVar x \<tau>1 # \<Gamma> \<turnstile> e : \<tau>2 \<rbrakk> \<Longrightarrow> \<Gamma> \<turnstile> (\<lambda> x : \<tau>1 . e) : (\<tau>1 \<rightarrow> \<tau>2)"
 
 | T_AppI: "\<lbrakk> \<Gamma> \<turnstile> e1 : (\<tau>1 \<rightarrow> \<tau>2) ; \<Gamma> \<turnstile> e2 : \<tau>1 \<rbrakk> \<Longrightarrow> \<Gamma> \<turnstile> App e1 e2 : \<tau>2"
 
-| T_LetI: "\<lbrakk> atom x \<sharp> (\<Gamma>, e1) ; \<Gamma> \<turnstile>\<^sub>t\<^sub>y \<tau>1 ; BVar x \<tau>1 # \<Gamma> \<turnstile> e2 : \<tau>2 ; \<Gamma> \<turnstile> e1 : \<tau>1 \<rbrakk> \<Longrightarrow> \<Gamma> \<turnstile> Let x \<tau>1 e1 e2 : \<tau>2"
+| T_LetI: "\<lbrakk> atom x \<sharp> (\<Gamma>, e1) ; \<Gamma> \<turnstile>\<^sub>t\<^sub>y \<tau>1 : \<star> ; BVar x \<tau>1 # \<Gamma> \<turnstile> e2 : \<tau>2 ; \<Gamma> \<turnstile> e1 : \<tau>1 \<rbrakk> \<Longrightarrow> \<Gamma> \<turnstile> Let x \<tau>1 e1 e2 : \<tau>2"
 
-| T_AppTI: "\<lbrakk> \<Gamma> \<turnstile> e : (\<forall>a . \<sigma>) ; \<Gamma> \<turnstile>\<^sub>t\<^sub>y \<tau> \<rbrakk> \<Longrightarrow> \<Gamma> \<turnstile> TyApp e \<tau> : subst_type \<tau> a \<sigma>"
+| T_AppTI: "\<lbrakk> \<Gamma> \<turnstile> e : (\<forall>a : k . \<sigma>) ; \<Gamma> \<turnstile>\<^sub>t\<^sub>y \<tau> : k \<rbrakk> \<Longrightarrow> \<Gamma> \<turnstile> TyApp e \<tau> : subst_type \<tau> a \<sigma>"
 
-| T_AbsTI: "\<lbrakk> BTyVar a # \<Gamma> \<turnstile> e : \<sigma> ; atom a \<sharp> \<Gamma> \<rbrakk> \<Longrightarrow> \<Gamma> \<turnstile> (\<Lambda> a . e) : (\<forall> a . \<sigma>)"
+| T_AbsTI: "\<lbrakk> BTyVar a k # \<Gamma> \<turnstile> e : \<sigma> ; atom a \<sharp> \<Gamma> \<rbrakk> \<Longrightarrow> \<Gamma> \<turnstile> (\<Lambda> a : k . e) : (\<forall> a : k . \<sigma>)"
 equivariance T
 nominal_inductive T avoids
   T_AbsI: x
