Soundness.thy
@@ -24,7 +24,7 @@ case (T_AppI e1 \<tau>1 \<tau>2 e2)
       then show ?thesis by simp
     next
       assume "\<exists>e2'. Step e2 e2'"
-      then show ?thesis using ST_BetaI T_AppI.hyps(1) \<open>is_value e1\<close> fun_ty_lam by blast 
+      then show ?thesis using ST_BetaI T_AppI.hyps(1) \<open>is_value e1\<close> fun_ty_lam by blast
     qed
   next
     assume "\<exists>e1'. Step e1 e1'"
@@ -40,8 +40,8 @@ next
   from T_AppTI(2) show ?case
   proof (elim disjE)
     assume "is_value e"
-    then obtain b e1 where "e = (\<Lambda> b . e1)" using T_AppTI
-      by (smt T.cases \<tau>.distinct(11) \<tau>.distinct(5) is_value.simps(1) is_value.simps(4) is_value.simps(5) is_value.simps(7))
+    then obtain b k e1 where "e = (\<Lambda> b : k . e1)" using T_AppTI
+      by (smt T.simps \<tau>.distinct(17) \<tau>.distinct(7) is_value.simps(1) is_value.simps(4) is_value.simps(5) is_value.simps(7))
     then show ?thesis using Step.ST_BetaTI T_AppTI by blast
   next
     assume "\<exists>e'. Step e e'"
@@ -50,23 +50,26 @@ next
 qed auto
 
 lemma context_invariance_ty:
-  assumes "\<Gamma> \<turnstile>\<^sub>t\<^sub>y \<tau>"
-  and has_tyvars: "\<forall>a. Set.member (atom a) (fv_\<tau> \<tau>) \<and> BTyVar a \<in> \<Gamma> \<longrightarrow> BTyVar a \<in> \<Gamma>'"
-  shows "\<Gamma>' \<turnstile>\<^sub>t\<^sub>y \<tau>"
-using assms proof (nominal_induct \<Gamma> \<tau> avoiding: \<Gamma>' rule: Ty.strong_induct)
+  assumes "\<Gamma> \<turnstile>\<^sub>t\<^sub>y \<tau> : k"
+  and has_tyvars: "\<forall>a k. Set.member (atom a) (fv_\<tau> \<tau>) \<and> BTyVar a k \<in> \<Gamma> \<longrightarrow> BTyVar a k \<in> \<Gamma>'"
+  shows "\<Gamma>' \<turnstile>\<^sub>t\<^sub>y \<tau> : k"
+using assms proof (nominal_induct \<Gamma> \<tau> k avoiding: \<Gamma>' rule: Ty.strong_induct)
   case (Ty_Var a \<Gamma>)
   then show ?case using supp_at_base Ty.Ty_Var by fastforce
+next
+  case (Ty_App \<Gamma> \<tau>1 \<kappa>1 \<kappa>2 \<tau>2)
+  then show ?case by (metis Ty.Ty_App UnCI \<tau>.fv_defs(4))
 qed (auto intro: Ty.intros)
 
 lemma context_invariance:
   assumes "\<Gamma> \<turnstile> e : \<tau>"
   and has_vars: "\<forall>x \<tau>'. Set.member (atom x) (fv_term e) \<and> BVar x \<tau>' \<in> \<Gamma> \<longrightarrow> BVar x \<tau>' \<in> \<Gamma>'"
-  and has_tyvars: "\<forall>a. Set.member (atom a) (fv_term e) \<and> BTyVar a \<in> \<Gamma> \<longrightarrow> BTyVar a \<in> \<Gamma>'"
+  and has_tyvars: "\<forall>a k. Set.member (atom a) (fv_term e) \<and> BTyVar a k \<in> \<Gamma> \<longrightarrow> BTyVar a k \<in> \<Gamma>'"
   shows "\<Gamma>' \<turnstile> e : \<tau>"
 using assms proof (nominal_induct \<Gamma> e \<tau> avoiding: \<Gamma>' rule: T.strong_induct)
   case (T_AbsI x \<Gamma> \<tau>1 e \<tau>2)
   then have 1: "BVar x \<tau>1 # \<Gamma>' \<turnstile> e : \<tau>2" by auto
-  have 2: "\<Gamma>' \<turnstile>\<^sub>t\<^sub>y \<tau>1" using context_invariance_ty[OF T_AbsI(3)] T_AbsI(7) fv_supp_subset by auto
+  have 2: "\<Gamma>' \<turnstile>\<^sub>t\<^sub>y \<tau>1 : \<star>" using context_invariance_ty[OF T_AbsI(3)] T_AbsI(7) fv_supp_subset by (simp add: subset_eq)
   show ?case by (rule T.T_AbsI[OF T_AbsI(1) 2 1])
 next
   case (T_AppI \<Gamma> e1 \<tau>1 \<tau>2 e2)
@@ -76,16 +79,16 @@ next
   then have 1: "BVar x \<tau>1 # \<Gamma>' \<turnstile> e2 : \<tau>2" by auto
   from T_LetI have 2: "atom x \<sharp> (\<Gamma>', e1)" by auto
   from T_LetI have 3: "\<Gamma>' \<turnstile> e1 : \<tau>1" by force
-  have 4: "\<Gamma>' \<turnstile>\<^sub>t\<^sub>y \<tau>1" using context_invariance_ty[OF T_LetI(4)] T_LetI(10) fv_supp_subset by auto
+  have 4: "\<Gamma>' \<turnstile>\<^sub>t\<^sub>y \<tau>1 : \<star>" using context_invariance_ty[OF T_LetI(4)] T_LetI(10) fv_supp_subset by (simp add: subset_eq)
   show ?case by (rule T.T_LetI[OF 2 4 1 3])
 next
-  case (T_AppTI \<Gamma> e a \<sigma> \<tau>)
-  then have 1: "\<Gamma>' \<turnstile> e : \<forall> a . \<sigma>" by simp
-  have 2: "\<Gamma>' \<turnstile>\<^sub>t\<^sub>y \<tau>" using context_invariance_ty[OF T_AppTI(3)] T_AppTI(5) fv_supp_subset by auto
+  case (T_AppTI \<Gamma> e a k \<sigma> \<tau>)
+  then have 1: "\<Gamma>' \<turnstile> e : \<forall> a : k . \<sigma>" by simp
+  have 2: "\<Gamma>' \<turnstile>\<^sub>t\<^sub>y \<tau> : k" using context_invariance_ty[OF T_AppTI(3)] T_AppTI(5) fv_supp_subset by (simp add: subset_eq)
   show ?case by (rule T.T_AppTI[OF 1 2])
 next
-  case (T_AbsTI a \<Gamma> e \<sigma>)
-  then have 1: "BTyVar a # \<Gamma>' \<turnstile> e : \<sigma>" by auto
+  case (T_AbsTI a k \<Gamma> e \<sigma>)
+  then have 1: "BTyVar a k # \<Gamma>' \<turnstile> e : \<sigma>" by auto
   have 2: "atom a \<sharp> \<Gamma>'" using T_AbsTI by auto
   show ?case by (rule T.T_AbsTI[OF 1 2])
 qed (auto intro: T.intros simp: supp_at_base)
@@ -121,65 +124,88 @@ next
 next
   case (Lam y \<sigma> e')
   then have 1: "atom y \<sharp> BVar x \<tau>' # \<Gamma>" by (simp add: fresh_Cons)
-  obtain \<tau>2 where P: "BVar y \<sigma> # BVar x \<tau>' # \<Gamma> \<turnstile> e' : \<tau>2" "\<tau> = (\<sigma> \<rightarrow> \<tau>2)" "BVar x \<tau>' # \<Gamma> \<turnstile>\<^sub>t\<^sub>y \<sigma>" using T_Abs_Inv[OF Lam(7) 1] by blast
+  obtain \<tau>2 where P: "BVar y \<sigma> # BVar x \<tau>' # \<Gamma> \<turnstile> e' : \<tau>2" "\<tau> = (\<sigma> \<rightarrow> \<tau>2)" "BVar x \<tau>' # \<Gamma> \<turnstile>\<^sub>t\<^sub>y \<sigma> : \<star>" using T_Abs_Inv[OF Lam(7) 1] by blast
   then have 2: "BVar x \<tau>' # BVar y \<sigma> # \<Gamma> \<turnstile> e' : \<tau>2" using Lam(4) context_invariance by auto
-  from P have 3: "\<Gamma> \<turnstile>\<^sub>t\<^sub>y \<sigma>" using context_invariance_ty by auto
+  from P have 3: "\<Gamma> \<turnstile>\<^sub>t\<^sub>y \<sigma> : \<star>" using context_invariance_ty by auto
   from Lam show ?case using T.T_AbsI[OF Lam(1) 3] P 2 by auto
 next
-  case (TyLam a e)
+  case (TyLam a k e)
   have 1: "atom a \<sharp> BVar x \<tau>' # \<Gamma>" by (simp add: TyLam.hyps(1) TyLam.hyps(5) fresh_Cons)
-  obtain \<sigma> where P: "BTyVar a # BVar x \<tau>' # \<Gamma> \<turnstile> e : \<sigma>" "\<tau> = (\<forall> a . \<sigma>)" using T_AbsT_Inv[OF TyLam(7) 1 TyLam(2)] by blast
-  then have 1: "BVar x \<tau>' # BTyVar a # \<Gamma> \<turnstile> e : \<sigma>" using context_invariance by fastforce
-  have 2: "BTyVar a # \<Gamma> \<turnstile> subst_term v x e : \<sigma>" by (rule TyLam(6)[OF 1 TyLam(8)])
+  obtain \<sigma> where P: "BTyVar a k # BVar x \<tau>' # \<Gamma> \<turnstile> e : \<sigma>" "\<tau> = (\<forall> a : k . \<sigma>)" using T_AbsT_Inv[OF TyLam(7) 1 TyLam(2)] by blast
+  then have 1: "BVar x \<tau>' # BTyVar a k # \<Gamma> \<turnstile> e : \<sigma>" using context_invariance by fastforce
+  have 2: "BTyVar a k # \<Gamma> \<turnstile> subst_term v x e : \<sigma>" by (rule TyLam(6)[OF 1 TyLam(8)])
   from TyLam show ?case using T.T_AbsTI[OF 2 TyLam(1)] P by auto
 next
   case (Let y \<tau>1 e1 e2)
   then have 1: "atom y \<sharp> BVar x \<tau>' # \<Gamma>" by (simp add: fresh_Cons)
-  have P: "BVar x \<tau>' # \<Gamma> \<turnstile> e1 : \<tau>1" "BVar y \<tau>1 # BVar x \<tau>' # \<Gamma> \<turnstile> e2 : \<tau>" "BVar x \<tau>' # \<Gamma> \<turnstile>\<^sub>t\<^sub>y \<tau>1" using T_Let_Inv[OF Let(8) 1] by auto
+  have P: "BVar x \<tau>' # \<Gamma> \<turnstile> e1 : \<tau>1" "BVar y \<tau>1 # BVar x \<tau>' # \<Gamma> \<turnstile> e2 : \<tau>" "BVar x \<tau>' # \<Gamma> \<turnstile>\<^sub>t\<^sub>y \<tau>1 : \<star>" using T_Let_Inv[OF Let(8) 1] by auto
   have 2: "\<Gamma> \<turnstile> subst_term v x e1 : \<tau>1" by (rule Let(6)[OF P(1) Let(9)])
   have 3: "BVar x \<tau>' # BVar y \<tau>1 # \<Gamma> \<turnstile> e2 : \<tau>" using Let(4) P(2) context_invariance by auto
   have 4: "BVar y \<tau>1 # \<Gamma> \<turnstile> subst_term v x e2 : \<tau>" by (rule Let(7)[OF 3 Let(9)])
-  have 5: "\<Gamma> \<turnstile>\<^sub>t\<^sub>y \<tau>1" using context_invariance_ty[OF P(3)] by auto
+  have 5: "\<Gamma> \<turnstile>\<^sub>t\<^sub>y \<tau>1 : \<star>" using context_invariance_ty[OF P(3)] by auto
   have "atom y \<sharp> subst_term v x e1" using "2" Let(1) fresh_term_var by blast
   then have 6: "atom y \<sharp> (\<Gamma>, subst_term v x e1)" using Let(1) by auto
   show ?case using T.T_LetI[OF 6 5 4 2] Let by auto
 qed
 
-lemma type_substitution_ty: "\<lbrakk> BTyVar a # \<Gamma> \<turnstile>\<^sub>t\<^sub>y \<tau> ; \<Gamma> \<turnstile>\<^sub>t\<^sub>y \<tau>' ; atom a \<sharp> \<Gamma> \<rbrakk> \<Longrightarrow> \<Gamma> \<turnstile>\<^sub>t\<^sub>y subst_type \<tau>' a \<tau>"
-proof (nominal_induct \<tau> avoiding: a \<Gamma> \<tau>' rule: \<tau>.strong_induct)
+lemma type_substitution_ty: "\<lbrakk> BTyVar a k # \<Gamma> \<turnstile>\<^sub>t\<^sub>y \<tau> : k2 ; \<Gamma> \<turnstile>\<^sub>t\<^sub>y \<tau>' : k ; atom a \<sharp> \<Gamma> \<rbrakk> \<Longrightarrow> \<Gamma> \<turnstile>\<^sub>t\<^sub>y subst_type \<tau>' a \<tau> : k2"
+proof (nominal_induct \<tau> avoiding: a \<Gamma> \<tau>' k k2 rule: \<tau>.strong_induct)
+ case TyUnit
+  then show ?case using context_invariance_ty by auto
+next
   case (TyVar x)
-  then show ?case by (metis \<tau>.fv_defs(2) atom_eq_iff context_invariance_ty empty_iff insertE isin.simps(5) subst_type.simps(2) supp_at_base)
+  then show ?case
+  proof (cases "atom x = atom a")
+    case True
+    then have "k = k2" using Ty.cases TyVar.prems(1) by force
+    then show ?thesis using TyVar True by auto
+  next
+    case False
+    then show ?thesis
+      by (smt TyVar.prems(1) TyVar.prems(2) TyVar.prems(3) \<tau>.fv_defs(2) \<tau>.supp(2) context_invariance_ty fresh_def fresh_subst_type isin.simps(5) subst_type.simps(2) ty_fresh_vars)
+  qed
 next
   case (TyArrow e1 e2)
-  then show ?case by (metis Ty.simps \<tau>.distinct(11) \<tau>.distinct(3) \<tau>.distinct(7) \<tau>.eq_iff(3) subst_type.simps(3))
+  then have 1: "k2 = \<star>" using Ty.cases[OF TyArrow(3)] by (smt \<tau>.distinct(15) \<tau>.distinct(9))
+  then have "BTyVar a k # \<Gamma> \<turnstile>\<^sub>t\<^sub>y e1 : \<star>" "BTyVar a k # \<Gamma> \<turnstile>\<^sub>t\<^sub>y e2 : \<star>" using Ty.cases[OF TyArrow(3)] by auto
+  then show ?case using TyArrow 1 Ty_Arrow by auto
 next
-  case (TyForall b \<tau>)
-  have "BTyVar b # BTyVar a # \<Gamma> \<turnstile>\<^sub>t\<^sub>y \<tau>" proof (cases rule: Ty.cases[OF TyForall(5)])
-    case (4 c \<Gamma> \<sigma>)
-    then have "\<tau> = (b \<leftrightarrow> c) \<bullet> \<sigma>" by (metis Abs1_eq_iff(3) TyForall.prems(1) \<tau>.eq_iff(4) \<tau>.perm_simps(4) flip_at_simps(2) flip_fresh_fresh ty_fresh_vars)
-    then show ?thesis
-      by (smt "4"(1) "4"(3) "4"(4) Cons_eqvt Ty.eqvt TyForall.hyps(1) TyForall.hyps(2) binder.fresh(2) binder.perm_simps(2) flip_at_simps(2) flip_def fresh_Cons swap_fresh_fresh)
+  case (TyConApp \<tau>1 \<tau>2)
+  then obtain k1 where "BTyVar a k # \<Gamma> \<turnstile>\<^sub>t\<^sub>y \<tau>1 : KArrow k1 k2 \<and> BTyVar a k # \<Gamma> \<turnstile>\<^sub>t\<^sub>y \<tau>2 : k1" using Ty.cases[OF TyConApp(3)] by fastforce
+  then show ?case using TyConApp Ty_App by fastforce
+next
+  case (TyForall b k3 \<tau>)
+  then have "k2 = \<star>" using Ty.cases by fastforce
+  have "BTyVar b k3 # BTyVar a k # \<Gamma> \<turnstile>\<^sub>t\<^sub>y \<tau> : \<star>" proof (cases rule: Ty.cases[OF TyForall(7)])
+    case (5 c k4 \<Gamma>2 \<sigma>)
+    then have 1: "\<tau> = (b \<leftrightarrow> c) \<bullet> \<sigma>" by (smt Abs1_eq_iff(3) TyForall.prems(1) \<tau>.eq_iff(5) \<tau>.perm_simps(5) flip_at_simps(2) flip_def swap_fresh_fresh ty_fresh_vars)
+    from 5 have "k4 = k3" by auto
+    then have "(b \<leftrightarrow> c) \<bullet> (BTyVar c k3 # \<Gamma>2 \<turnstile>\<^sub>t\<^sub>y \<sigma> : \<star>)" using 5(4) by simp
+    then have 2: "((b \<leftrightarrow> c) \<bullet> BTyVar c k3) # \<Gamma>2 \<turnstile>\<^sub>t\<^sub>y (b \<leftrightarrow> c) \<bullet> \<sigma> : \<star>" by (smt "5"(1) "5"(4) "5"(5) Cons_eqvt Ty.eqvt TyForall.hyps(1) TyForall.hyps(2) TyForall.hyps(4) \<kappa>.perm_simps(1) \<open>k4 = k3\<close> binder.fresh(2) flip_def fresh_Cons swap_fresh_fresh)
+    have "(b \<leftrightarrow> c) \<bullet> BTyVar c k3 = BTyVar b k3" by (simp add: flip_def swap_fresh_fresh)
+    then show ?thesis using 1 2 5(1) by argo
   qed auto
-  then have 1: "BTyVar a # BTyVar b # \<Gamma> \<turnstile>\<^sub>t\<^sub>y \<tau>" using context_invariance_ty by auto
-  show ?case
-    by (metis (mono_tags, lifting) "1" Ty.simps TyForall.hyps(1) TyForall.hyps(2) TyForall.hyps(3) TyForall.hyps(4) TyForall.prems(2) TyForall.prems(3) binder.supp(2) context_invariance_ty fresh_Cons fresh_Pair fresh_def isin.simps(5) singletonD subst_type.simps(4) supp_at_base)
-qed (auto intro: Ty.intros)
+  then have 1: "BTyVar a k # BTyVar b k3 # \<Gamma> \<turnstile>\<^sub>t\<^sub>y \<tau> : \<star>" using context_invariance_ty TyForall(1) by auto
+  have 2: "BTyVar b k3 # \<Gamma> \<turnstile>\<^sub>t\<^sub>y \<tau>' : k" using context_invariance_ty[OF TyForall(8)] by (simp add: TyForall.hyps(2) fresh_not_isin_tyvar)
+  have 3: "BTyVar b k3 # \<Gamma> \<turnstile>\<^sub>t\<^sub>y subst_type \<tau>' a \<tau> : \<star>" using TyForall(6)[OF 1 2] using TyForall.hyps(1) TyForall.prems(3) fresh_Cons by fastforce
+  then show ?case by (simp add: TyForall.hyps(1) TyForall.hyps(2) TyForall.hyps(3) Ty_Forall \<open>k2 = \<star>\<close>)
+qed
 
 lemma type_substitution:
-  assumes well_typed: "BTyVar a # \<Gamma> \<turnstile> e : \<sigma>" "\<Gamma> \<turnstile>\<^sub>t\<^sub>y \<tau>'"
-  and context_tyvar: "\<forall>b. BTyVar b \<in> \<Gamma> \<longrightarrow> BTyVar b \<in> \<Gamma>'"
+  assumes well_typed: "BTyVar a k # \<Gamma> \<turnstile> e : \<sigma>" "\<Gamma> \<turnstile>\<^sub>t\<^sub>y \<tau>' : k"
+  and context_tyvar: "\<forall>b k. BTyVar b k \<in> \<Gamma> \<longrightarrow> BTyVar b k \<in> \<Gamma>'"
   and context_var: "\<forall>x \<tau>. BVar x \<tau> \<in> \<Gamma> \<longrightarrow> BVar x (subst_type \<tau>' a \<tau>) \<in> \<Gamma>'"
   and fresh: "atom a \<sharp> \<Gamma>'"
 shows "\<Gamma>' \<turnstile> subst_term_type \<tau>' a e : subst_type \<tau>' a \<sigma>"
-using assms proof (nominal_induct e avoiding: a \<Gamma> \<Gamma>' \<sigma> \<tau>' rule: term.strong_induct)
+using assms proof (nominal_induct e avoiding: a k \<Gamma> \<Gamma>' \<sigma> \<tau>' rule: term.strong_induct)
   case (Var x)
   then have 1: "BVar x (subst_type \<tau>' a \<sigma>) \<in> \<Gamma>'"
     by (smt T.cases isin.simps(3) term.distinct(1) term.distinct(11) term.distinct(3) term.distinct(5) term.distinct(7) term.distinct(9) term.eq_iff(1))
   show ?case using T.T_VarI[OF 1] by simp
 next
   case (App e1 e2)
-  obtain \<tau>1 where "BTyVar a # \<Gamma> \<turnstile> e1 : (\<tau>1 \<rightarrow> \<sigma>) \<and> BTyVar a # \<Gamma> \<turnstile> e2 : \<tau>1" using T.cases[OF App(3)] by fastforce
-  then have P: "BTyVar a # \<Gamma> \<turnstile> e1 : (\<tau>1 \<rightarrow> \<sigma>)" "BTyVar a # \<Gamma> \<turnstile> e2 : \<tau>1" by auto
+  obtain \<tau>1 where "BTyVar a k # \<Gamma> \<turnstile> e1 : (\<tau>1 \<rightarrow> \<sigma>) \<and> BTyVar a k # \<Gamma> \<turnstile> e2 : \<tau>1" using T.cases[OF App(3)] by fastforce
+  then have P: "BTyVar a k # \<Gamma> \<turnstile> e1 : (\<tau>1 \<rightarrow> \<sigma>)" "BTyVar a k # \<Gamma> \<turnstile> e2 : \<tau>1" by auto
 
   have 1: "\<Gamma>' \<turnstile> subst_term_type \<tau>' a e1 : subst_type \<tau>' a \<tau>1 \<rightarrow> subst_type \<tau>' a \<sigma>" using App(1)[OF P(1) App(4) App(5) App(6) App(7)] by simp
   have 2: "\<Gamma>' \<turnstile> subst_term_type \<tau>' a e2 : subst_type \<tau>' a \<tau>1" by (rule App(2)[OF P(2) App(4) App(5) App(6) App(7)])
@@ -188,22 +214,22 @@ next
 next
   case (TyApp e \<tau>)
 
-  have "\<exists>b \<sigma>'. BTyVar a # \<Gamma> \<turnstile> e : (\<forall>b . \<sigma>') \<and> atom b \<sharp> a \<and> \<sigma> = subst_type \<tau> b \<sigma>' \<and> atom b \<sharp> \<tau>' \<and> BTyVar a # \<Gamma> \<turnstile>\<^sub>t\<^sub>y \<tau>"
+  have "\<exists>b k2 \<sigma>'. BTyVar a k # \<Gamma> \<turnstile> e : (\<forall>b : k2 . \<sigma>') \<and> atom b \<sharp> a \<and> \<sigma> = subst_type \<tau> b \<sigma>' \<and> atom b \<sharp> \<tau>' \<and> BTyVar a k # \<Gamma> \<turnstile>\<^sub>t\<^sub>y \<tau> : k2"
   proof (cases rule: T.cases[OF TyApp(2)])
-    case (6 \<Gamma>2 t b \<sigma>2 \<tau>2)
-    then have 1: "BTyVar a # \<Gamma> \<turnstile> e : \<forall> b . \<sigma>2" "\<sigma> = subst_type \<tau> b \<sigma>2" "BTyVar a # \<Gamma> \<turnstile>\<^sub>t\<^sub>y \<tau>" by auto
+    case (6 \<Gamma>2 t b k2 \<sigma>2 \<tau>2)
+    then have 1: "BTyVar a k # \<Gamma> \<turnstile> e : \<forall> b : k2 . \<sigma>2" "\<sigma> = subst_type \<tau> b \<sigma>2" "BTyVar a k # \<Gamma> \<turnstile>\<^sub>t\<^sub>y \<tau> : k2" by auto
     obtain c::tyvar where "atom c \<sharp> (a, b, \<sigma>2, \<tau>')" using obtain_fresh by blast
     then have c: "atom c \<sharp> b" "atom c \<sharp> \<sigma>2" "atom c \<sharp> a" "atom c \<sharp> \<tau>'" using fresh_Pair by auto
-    from 1(1) have 2: "BTyVar a # \<Gamma> \<turnstile> e : \<forall> c . (b \<leftrightarrow> c) \<bullet> \<sigma>2" by (smt Abs1_eq_iff(3) \<tau>.eq_iff(4) c(1) c(2) flip_commute fresh_at_base(2))
+    from 1(1) have 2: "BTyVar a k # \<Gamma> \<turnstile> e : \<forall> c : k2 . (b \<leftrightarrow> c) \<bullet> \<sigma>2" by (smt Abs1_eq_iff(3) \<tau>.eq_iff(5) c(1) c(2) flip_commute fresh_at_base(2))
     from 1(2) have "\<sigma> = subst_type \<tau> c ((b \<leftrightarrow> c) \<bullet> \<sigma>2)" using subst_type_var_name c by auto
     then show ?thesis using 2 c(3) c(4) 1(3) by blast
   qed auto
-  then obtain b \<sigma>' where P: "BTyVar a # \<Gamma> \<turnstile> e : (\<forall>b . \<sigma>')" "atom b \<sharp> a" "\<sigma> = subst_type \<tau> b \<sigma>'" "atom b \<sharp> \<tau>'" "BTyVar a # \<Gamma> \<turnstile>\<^sub>t\<^sub>y \<tau>" by blast
+  then obtain b k2 \<sigma>' where P: "BTyVar a k # \<Gamma> \<turnstile> e : (\<forall>b : k2 . \<sigma>')" "atom b \<sharp> a" "\<sigma> = subst_type \<tau> b \<sigma>'" "atom b \<sharp> \<tau>'" "BTyVar a k # \<Gamma> \<turnstile>\<^sub>t\<^sub>y \<tau> : k2" by blast
 
-  have 1: "\<Gamma>' \<turnstile>\<^sub>t\<^sub>y \<tau>'" using context_invariance_ty[OF TyApp(3)] using TyApp(5) TyApp.prems(3) by blast
-  have 2: "BTyVar a # \<Gamma>' \<turnstile>\<^sub>t\<^sub>y \<tau>" using context_invariance_ty[OF P(5)]by (smt TyApp.prems(3) isin.simps(5))
-  have 3: "\<Gamma>' \<turnstile>\<^sub>t\<^sub>y subst_type \<tau>' a \<tau>" by (rule type_substitution_ty[OF 2 1 TyApp(6)])
-  have 4: "\<Gamma>' \<turnstile> subst_term_type \<tau>' a e : \<forall> b . subst_type \<tau>' a \<sigma>'" using TyApp(1)[OF P(1) TyApp(3) TyApp(4) TyApp(5) TyApp(6)] P(2) P(4) by auto
+  have 1: "\<Gamma>' \<turnstile>\<^sub>t\<^sub>y \<tau>' : k" using context_invariance_ty[OF TyApp(3)] using TyApp.prems(3) by blast
+  have 2: "BTyVar a k # \<Gamma>' \<turnstile>\<^sub>t\<^sub>y \<tau> : k2" using context_invariance_ty[OF P(5)] by (smt TyApp.prems(3) isin.simps(5))
+  have 3: "\<Gamma>' \<turnstile>\<^sub>t\<^sub>y subst_type \<tau>' a \<tau> : k2" by (rule type_substitution_ty[OF 2 1 TyApp(6)])
+  have 4: "\<Gamma>' \<turnstile> subst_term_type \<tau>' a e : \<forall> b : k2 . subst_type \<tau>' a \<sigma>'" using TyApp(1)[OF P(1) TyApp(3) TyApp(4) TyApp(5) TyApp(6)] P(2) P(4) by auto
 
   have "\<Gamma>' \<turnstile> TyApp (subst_term_type \<tau>' a e) (subst_type \<tau>' a \<tau>) : subst_type \<tau>' a (subst_type \<tau> b \<sigma>')" using T.T_AppTI[OF 4 3] subst_type_order[OF P(4) P(2)] by simp
   then show ?case using P(3) by simp
@@ -213,46 +239,46 @@ next
   then show ?case using T.T_UnitI by simp
 next
   case (Lam x \<tau>1 e)
-  then have 1: "atom x \<sharp> BTyVar a # \<Gamma>" by (simp add: fresh_Cons)
-  obtain \<tau>2 where P: "BVar x \<tau>1 # BTyVar a # \<Gamma> \<turnstile> e : \<tau>2" "\<sigma> = (\<tau>1 \<rightarrow> \<tau>2)" "BTyVar a # \<Gamma> \<turnstile>\<^sub>t\<^sub>y \<tau>1" using T_Abs_Inv[OF Lam(7) 1] by blast
-  then have 2: "BTyVar a # BVar x \<tau>1 # \<Gamma> \<turnstile> e : \<tau>2" using context_invariance[OF P(1)] by simp
-  have 3: "BTyVar a # \<Gamma>' \<turnstile>\<^sub>t\<^sub>y \<tau>1" using context_invariance_ty[OF P(3)] by (smt Lam.prems(3) isin.simps(5))
-  have 4: "\<Gamma>' \<turnstile>\<^sub>t\<^sub>y \<tau>'" using context_invariance_ty[OF Lam(8)] using Lam.prems(3) by blast
-  have 5: "\<Gamma>' \<turnstile>\<^sub>t\<^sub>y subst_type \<tau>' a \<tau>1" by (simp add: "3" "4" Lam.prems(5) type_substitution_ty)
-  have 6: "BVar x \<tau>1 # \<Gamma> \<turnstile>\<^sub>t\<^sub>y \<tau>'" using context_invariance_ty[OF Lam(8)] Lam(9) by auto
+  then have 1: "atom x \<sharp> BTyVar a k # \<Gamma>" by (simp add: fresh_Cons)
+  obtain \<tau>2 where P: "BVar x \<tau>1 # BTyVar a k # \<Gamma> \<turnstile> e : \<tau>2" "\<sigma> = (\<tau>1 \<rightarrow> \<tau>2)" "BTyVar a k # \<Gamma> \<turnstile>\<^sub>t\<^sub>y \<tau>1 : \<star>" using T_Abs_Inv[OF Lam(8) 1] by blast
+  then have 2: "BTyVar a k # BVar x \<tau>1 # \<Gamma> \<turnstile> e : \<tau>2" using context_invariance[OF P(1)] by simp
+  have 3: "BTyVar a k # \<Gamma>' \<turnstile>\<^sub>t\<^sub>y \<tau>1 : \<star>" using context_invariance_ty[OF P(3)] by (smt Lam.prems(3) isin.simps(5))
+  have 4: "\<Gamma>' \<turnstile>\<^sub>t\<^sub>y \<tau>' : k" using context_invariance_ty[OF Lam(9)] Lam.prems(3) by blast
+  have 5: "\<Gamma>' \<turnstile>\<^sub>t\<^sub>y subst_type \<tau>' a \<tau>1 : \<star>" using "3" "4" Lam.prems(5) type_substitution_ty by blast
+  have 6: "BVar x \<tau>1 # \<Gamma> \<turnstile>\<^sub>t\<^sub>y \<tau>' : k" using context_invariance_ty[OF Lam(9)] by auto
 
   from 4 have 7: "atom a \<sharp> \<tau>'" using Lam.prems(5) ty_fresh_vars by blast
   have 8: "atom a \<sharp> BVar x (subst_type \<tau>' a \<tau>1) # \<Gamma>'" using "5" Lam.prems(5) fresh_Cons ty_fresh_vars by fastforce
 
-  have 9: "BVar x (subst_type \<tau>' a \<tau>1) # \<Gamma>' \<turnstile> subst_term_type \<tau>' a e : subst_type \<tau>' a \<tau>2" using Lam(6)[OF 2 6 _ _ 8] by (simp add: Lam.prems(3) Lam.prems(4))
+  have 9: "BVar x (subst_type \<tau>' a \<tau>1) # \<Gamma>' \<turnstile> subst_term_type \<tau>' a e : subst_type \<tau>' a \<tau>2" using Lam(7)[OF 2 6 _ _ 8] by (simp add: Lam.prems(3) Lam.prems(4))
 
-  have "\<Gamma>' \<turnstile> \<lambda>x : subst_type \<tau>' a \<tau>1 . subst_term_type \<tau>' a e : subst_type \<tau>' a \<tau>1 \<rightarrow> subst_type \<tau>' a \<tau>2" using T.T_AbsI[OF Lam(3) 5 9] .
+  have "\<Gamma>' \<turnstile> \<lambda>x : subst_type \<tau>' a \<tau>1 . subst_term_type \<tau>' a e : subst_type \<tau>' a \<tau>1 \<rightarrow> subst_type \<tau>' a \<tau>2" by (rule T.T_AbsI[OF Lam(4) 5 9])
   then show ?case using P(2) by simp
 next
-  case (TyLam b e)
-  then have 1: "atom b \<sharp> BTyVar a # \<Gamma>" by (simp add: fresh_Cons)
-  obtain \<tau> where P: "BTyVar b # BTyVar a # \<Gamma> \<turnstile> e : \<tau>" "\<sigma> = (\<forall> b . \<tau>)" using T_AbsT_Inv[OF TyLam(7) 1 TyLam(4)] by blast
-  then have 2: "subst_type \<tau>' a \<sigma> = (\<forall> b . subst_type \<tau>' a \<tau>)" by (simp add: TyLam(1) TyLam(5))
-  have 3: "BTyVar a # BTyVar b # \<Gamma> \<turnstile> e : \<tau>" using context_invariance[OF P(1)] TyLam(9) TyLam(10) by auto
-  have 4: "BTyVar b # \<Gamma> \<turnstile>\<^sub>t\<^sub>y \<tau>'" using context_invariance_ty[OF TyLam(8)] by simp
-  have 5: "atom a \<sharp> BTyVar b # \<Gamma>'" using TyLam(1) TyLam.prems(5) fresh_Cons by fastforce
+  case (TyLam b k2 e)
+  then have 1: "atom b \<sharp> BTyVar a k # \<Gamma>" by (simp add: fresh_Cons)
+  obtain \<tau> where P: "BTyVar b k2 # BTyVar a k # \<Gamma> \<turnstile> e : \<tau>" "\<sigma> = (\<forall> b : k2 . \<tau>)" using T_AbsT_Inv[OF TyLam(8) 1 TyLam(5)] by blast
+  then have 2: "subst_type \<tau>' a \<sigma> = (\<forall> b : k2 . subst_type \<tau>' a \<tau>)" by (simp add: TyLam(1) TyLam(6))
+  have 3: "BTyVar a k # BTyVar b k2 # \<Gamma> \<turnstile> e : \<tau>" using context_invariance[OF P(1)] by (smt TyLam.hyps(1) fresh_at_base(2) isin.simps(3) isin.simps(5))
+  have 4: "BTyVar b k2 # \<Gamma> \<turnstile>\<^sub>t\<^sub>y \<tau>' : k" using context_invariance_ty[OF TyLam(9)] by (simp add: TyLam.hyps(3) fresh_not_isin_tyvar)
+  have 5: "atom a \<sharp> BTyVar b k2 # \<Gamma>'" using TyLam(1) TyLam.prems(5) fresh_Cons by fastforce
 
-  have 9: "BTyVar b # \<Gamma>' \<turnstile> subst_term_type \<tau>' a e : subst_type \<tau>' a \<tau>" using TyLam(6)[OF 3 4 _ _ 5] TyLam(9) TyLam(10) by simp
+  have 9: "BTyVar b k2 # \<Gamma>' \<turnstile> subst_term_type \<tau>' a e : subst_type \<tau>' a \<tau>" using TyLam(7)[OF 3 4 _ _ 5] TyLam(10) TyLam(11) by simp
 
-  show ?case using T.T_AbsTI[OF 9 TyLam(3)] 2 TyLam(1) TyLam(5) by simp
+  show ?case using T.T_AbsTI[OF 9 TyLam(4)] 2 TyLam(1) TyLam(6) by simp
 next
   case (Let x \<tau>1 e1 e2)
-  then have 1: "atom x \<sharp> BTyVar a # \<Gamma>" by (simp add: fresh_Cons)
-  have P: "BTyVar a # \<Gamma> \<turnstile> e1 : \<tau>1" "BVar x \<tau>1 # BTyVar a # \<Gamma> \<turnstile> e2 : \<sigma>" "BTyVar a # \<Gamma> \<turnstile>\<^sub>t\<^sub>y \<tau>1" using T_Let_Inv[OF Let(8) 1] by auto
+  then have 1: "atom x \<sharp> BTyVar a k # \<Gamma>" by (simp add: fresh_Cons)
+  have P: "BTyVar a k # \<Gamma> \<turnstile> e1 : \<tau>1" "BVar x \<tau>1 # BTyVar a k # \<Gamma> \<turnstile> e2 : \<sigma>" "BTyVar a k # \<Gamma> \<turnstile>\<^sub>t\<^sub>y \<tau>1 : \<star>" using T_Let_Inv[OF Let(9) 1] by auto
   have 2: "atom x \<sharp> e1" using "1" P(1) fresh_term_var by blast
   have "atom x \<sharp> subst_term_type \<tau>' a e1" using Let P(1) fresh_term_var by blast
-  then have 3: "atom x \<sharp> (\<Gamma>', subst_term_type \<tau>' a e1)" using Let(3) by simp
-  have 4: "\<Gamma>' \<turnstile>\<^sub>t\<^sub>y subst_type \<tau>' a \<tau>1" using Let P(3) context_invariance_ty isin.simps(5) type_substitution_ty by presburger
+  then have 3: "atom x \<sharp> (\<Gamma>', subst_term_type \<tau>' a e1)" using Let(4) by simp
+  have 4: "\<Gamma>' \<turnstile>\<^sub>t\<^sub>y subst_type \<tau>' a \<tau>1 : \<star>" by (smt Let.prems(2) Let.prems(3) Let.prems(5) P(3) context_invariance_ty isin.simps(5) type_substitution_ty)
   have 5: "atom a \<sharp> BVar x (subst_type \<tau>' a \<tau>1) # \<Gamma>'" using "4" Let.prems(5) fresh_Cons ty_fresh_vars by fastforce
-  have 6: "BTyVar a # BVar x \<tau>1 # \<Gamma> \<turnstile> e2 : \<sigma>" using context_invariance[OF P(2)] by auto
-  have 7: "BVar x \<tau>1 # \<Gamma> \<turnstile>\<^sub>t\<^sub>y \<tau>'" using Let.prems(2) context_invariance_ty isin.simps(4) by blast
+  have 6: "BTyVar a k # BVar x \<tau>1 # \<Gamma> \<turnstile> e2 : \<sigma>" using context_invariance[OF P(2)] by auto
+  have 7: "BVar x \<tau>1 # \<Gamma> \<turnstile>\<^sub>t\<^sub>y \<tau>' : k" using Let.prems(2) context_invariance_ty isin.simps(4) by blast
 
-  have 9: "BVar x (subst_type \<tau>' a \<tau>1) # \<Gamma>' \<turnstile> subst_term_type \<tau>' a e2 : subst_type \<tau>' a \<sigma>" using Let(7)[OF 6 7 _ _ 5] Let(10) Let(11) by simp
+  have 9: "BVar x (subst_type \<tau>' a \<tau>1) # \<Gamma>' \<turnstile> subst_term_type \<tau>' a e2 : subst_type \<tau>' a \<sigma>" using Let(8)[OF 6 7 _ _ 5] Let(11) Let(12) by simp
   show ?case using T.T_LetI[OF 3 4 9] using Let P(1) by auto
 qed
 
@@ -301,30 +327,35 @@ next
     qed
   qed
 next
-  case (T_AppTI e a \<sigma> \<tau>)
+  case (T_AppTI e a k \<sigma> \<tau>)
   from T_AppTI(4) show ?case
   proof cases
-    case (ST_BetaTI b t)
+    case (ST_BetaTI b k2 t)
     obtain c::tyvar where "atom c \<sharp> (a, b, t, \<sigma>)" using obtain_fresh by blast
     then have c: "atom c \<sharp> a" "atom c \<sharp> b" "atom c \<sharp> t" "atom c \<sharp> \<sigma>" using fresh_Pair by auto
-    have 1: "[] \<turnstile> (\<Lambda> c . (b \<leftrightarrow> c) \<bullet> t) : \<forall> c . (a \<leftrightarrow> c) \<bullet> \<sigma>" by (smt Abs_lst_rename T_AppTI.hyps(1) \<tau>.eq_iff(4) atom_tyvar_sort c(3) c(4) local.ST_BetaTI(1) term.eq_iff(6))
+    have 1: "[] \<turnstile> (\<Lambda> c : k2 . (b \<leftrightarrow> c) \<bullet> t) : \<forall> c : k2 . (a \<leftrightarrow> c) \<bullet> \<sigma>"
+      by (smt Abs1_eq_iff(3) T.cases T_AppTI.hyps(1) \<tau>.distinct(17) \<tau>.distinct(7) \<tau>.eq_iff(5) c(1) c(2) c(3) c(4) flip_commute fresh_at_base(2) is_value.simps(3) is_value.simps(4) is_value.simps(5) is_value.simps(7) isin.simps(1) local.ST_BetaTI(1) term.eq_iff(6))
 
-    have 2: "[BTyVar c] \<turnstile> (b \<leftrightarrow> c) \<bullet> t : (a \<leftrightarrow> c) \<bullet> \<sigma>"
+    have 2: "[BTyVar c k2] \<turnstile> (b \<leftrightarrow> c) \<bullet> t : (a \<leftrightarrow> c) \<bullet> \<sigma>"
     proof (cases rule: T.cases[OF 1])
-      case (7 a' \<Gamma> e \<sigma>')
+      case (7 a' k2' \<Gamma> e \<sigma>')
+      then have same: "k2 = k2'" using \<tau>.eq_iff(5) by blast
       have 1: "(b \<leftrightarrow> c) \<bullet> t = (a' \<leftrightarrow> c) \<bullet> e"
         by (metis (no_types, lifting) "7"(2) Abs1_eq_iff(3) Nominal2_Base.swap_self add_flip_cancel flip_commute flip_def permute_flip_cancel2 permute_plus term.eq_iff(6))
       have 2: "(a \<leftrightarrow> c) \<bullet> \<sigma> = (a' \<leftrightarrow> c) \<bullet> \<sigma>'"
-        by (smt "7"(3) Abs1_eq_iff(3) Nominal2_Base.swap_self \<tau>.eq_iff(4) c(4) flip_commute flip_def swap_fresh_fresh)
+        by (metis "7"(3) Abs1_eq_iff(3) Nominal2_Base.swap_self \<tau>.eq_iff(5) c(4) flip_commute flip_def swap_fresh_fresh)
+      from 7(4) have 3: "(a' \<leftrightarrow> c) \<bullet> (BTyVar a' k2' # \<Gamma> \<turnstile> e : \<sigma>')" by simp
+      have 4: "(a' \<leftrightarrow> c) \<bullet> (BTyVar a' k2' # \<Gamma>) = ((a' \<leftrightarrow> c) \<bullet> BTyVar a' k2') # \<Gamma>" using "7"(1) by auto
+      have 5: "(a' \<leftrightarrow> c) \<bullet> BTyVar a' k2' = BTyVar c k2'" using flip_fresh_fresh[OF no_tyvars_in_kinds[of a' k2'] no_tyvars_in_kinds[of c k2']] flip_at_base_simps(1)[of a' c] by simp
 
-      show ?thesis using 7(4) 1 2 by (smt "7"(1) Cons_eqvt Nil_eqvt T.eqvt binder.perm_simps(2) flip_at_simps(1))
+      show ?thesis using T.eqvt[OF 7(4), of "(a' \<leftrightarrow> c)"] using "1" "2" "5" "7"(1) same by auto
     qed auto
-
-    have "[] \<turnstile> subst_term_type \<tau> c ((b \<leftrightarrow> c) \<bullet> t) : subst_type \<tau> c ((a \<leftrightarrow> c) \<bullet> \<sigma>)" using type_substitution[OF 2 T_AppTI(3) _ _ fresh_Nil] by simp
+    have "k = k2" using T.cases T_AppTI.hyps(1) local.ST_BetaTI(1) by fastforce
+    then have "[] \<turnstile> subst_term_type \<tau> c ((b \<leftrightarrow> c) \<bullet> t) : subst_type \<tau> c ((a \<leftrightarrow> c) \<bullet> \<sigma>)" using type_substitution[OF 2 _ _ _ fresh_Nil] T_AppTI(3) by simp
     then show ?thesis using ST_BetaTI(2) subst_term_type_var_name[OF c(3)] subst_type_var_name[OF c(4)] by presburger
   next
     case (ST_AppTI e2)
-    then show ?thesis by (simp add: T.T_AppTI T_AppTI.hyps(2) T_AppTI.hyps(3))
+    then show ?thesis using T.T_AppTI T_AppTI.hyps(2) T_AppTI.hyps(3) by blast
   qed
 next
   case (T_AbsTI a e \<sigma>)
